More completed proofs, beginnings of indist encrypt, changed Term_const definition to take in a nat -> interp_term

src/Minimalistic.v
@@ -70,7 +70,7 @@ Section Language.
 
   Context {message list_message rand : base_type}.
   Inductive term : type -> Type :=
-  | Term_const {t} (_:interp_type t) : term t
+  | Term_const {t} (_: nat -> interp_type t) : term t
   | Term_random (_:nat) : term rand
   | Term_adversarial (_:term list_message) : term message
   | Term_app {dom cod} (_:term (Type_arrow dom cod)) (_:term dom) : term cod.
@@ -86,14 +86,15 @@ Section Language.
   Context (interp_random : nat -> interp_type rand).
   Context (interp_adversarial : interp_type list_message -> interp_type message).
   Fixpoint interp_term
-           {t} (e:term t) : interp_type t :=
+           {t} (e:term t) (eta : nat) : interp_type t :=
     match e with
-    | Term_const c => c
+    | Term_const c => c eta
     | Term_random n => interp_random n
-    | Term_adversarial ctx => interp_adversarial (interp_term ctx)
-    | Term_app f x => (interp_term f) (interp_term x)
+    | Term_adversarial ctx => interp_adversarial (interp_term ctx eta)
+    | Term_app f x => (interp_term f eta) (interp_term x eta)
     end.
 End Language.
+
 Arguments type : clear implicits.
 Arguments interp_type {_} _ _.
 Arguments term {_} _ _ _ _ _.
@@ -123,7 +124,7 @@ Section CompInterp.
           := List.firstn (rand_size eta) (List.skipn (n * rand_size eta) good_rand_tape) in
       let interp_adversarial : interp_type interp_base_type (Type_arrow (Type_base BaseType_list_message) (Type_base BaseType_message))
           := adversary eta evil_rand_tape in
-      interp_term interp_random interp_adversarial e.
+      interp_term interp_random interp_adversarial e eta.
 
     Definition universal_security_game eta {t:type base_type} (e:term t) : Comp bool :=
       good_rand_tape' <-$ {0,1}^(rand_end e * rand_size eta);
@@ -144,9 +145,6 @@ Section CompInterp.
     cbv [Reflexive indist]; setoid_rewrite ratDistance_0; eauto using negligible_0.
   Qed.
 
-  Print Reflexive.
-  Print Symmetric.
-
   Global Instance Symmetric_indist {t} : Symmetric (@indist t).
   Proof.
     cbv [Symmetric indist]; intros; setoid_rewrite ratDistance_comm; eauto.
@@ -159,79 +157,70 @@ Section CompInterp.
 
         (* dst : forall t : type base_type, nat -> list bool -> interp_type interp_base_type t -> bool, *)
 
-  Lemma not_indist_const {t} (x y : interp_type interp_base_type t) (tEqDec:forall x y : interp_type interp_base_type t, {x=y}+{x<>y}) (typeDec : forall x y : type base_type, {x=y}+{x<>y}) (H:x <> y) : ~indist (Term_const x) (Term_const y).
-  Proof.
-    cbv [indist].
-    intro X.
-    specialize (X id (fun _ _ _ => nil)
-                  ((fun t' => match typeDec t t' with
-                           | left pfeq => fun _ _ x' => ltac:(
-                                                      rewrite <- pfeq in x'; exact (if tEqDec x x' then true else false))
-                           | right pfne => fun _ _ _ => false
-                           end))).
+  (* Lemma not_indist_const {t} (x y : nat -> interp_type interp_base_type t) (tEqDec:forall x y : interp_type interp_base_type t, {x=y}+{x<>y}) (typeDec : forall x y : type base_type, {x=y}+{x<>y}) (H:x <> y) : ~indist (Term_const x) (Term_const y). *)
+  (* Proof. *)
+  (*   cbv [indist]. *)
+  (*   intro X. *)
+  (*   specialize (X id (fun _ _ _ => nil) *)
+  (*                 ((fun t' => match typeDec t t' with *)
+  (*                          | left pfeq => fun _ _ x' => ltac:( *)
+  (*                                                     rewrite <- pfeq in x'; exact (if tEqDec x x' then true else false)) *)
+  (*                          | right pfne => fun _ _ _ => false *)
+  (*                          end))). *)
 
-    cbv [universal_security_game comp_interp_term interp_term] in X.
-    destruct (typeDec t t) in X; [|congruence].
-    cbv [eq_rec_r eq_rec eq_rect eq_sym] in X.
-    replace e with (eq_refl:t=t) in X by admit.
+  (*   cbv [universal_security_game comp_interp_term interp_term] in X. *)
+  (*   destruct (typeDec t t) in X; [|congruence]. *)
+  (*   cbv [eq_rec_r eq_rec eq_rect eq_sym] in X. *)
+  (*   replace e with (eq_refl:t=t) in X by admit. *)
 
-    destruct (tEqDec x x) in X; [|congruence].
-    destruct (tEqDec x y) in X; [congruence|].
-    cbv[negligible] in X.
-    specialize (X 1%nat).
-    destruct X as [n' X].
-    specialize (X (1+n')%nat).
-    assert (nz (1+n')) by (constructor; omega).
-    specialize (X H0).
-    assert (1 + n' > n') by omega.
-    specialize (X H1).
-    apply X; clear X.
+  (*   destruct (tEqDec x x) in X; [|congruence]. *)
+  (*   destruct (tEqDec x y) in X; [congruence|]. *)
+  (*   cbv[negligible] in X. *)
+  (*   specialize (X 1%nat). *)
+  (*   destruct X as [n' X]. *)
+  (*   specialize (X (1+n')%nat). *)
+  (*   assert (nz (1+n')) by (constructor; omega). *)
+  (*   specialize (X H0). *)
+  (*   assert (1 + n' > n') by omega. *)
+  (*   specialize (X H1). *)
+  (*   apply X; clear X. *)
 
-    lazymatch goal with
-      |- context [ Pr [?C] ] =>
-      let H := fresh "H" in
-      assert (Pr [C] == 1) as H;
-        [|rewrite H; clear H]
-    end.
-    {
-      fcf_irr_l; fcf_well_formed; fcf_irr_l; fcf_well_formed; fcf_compute.
-    }
+  (*   lazymatch goal with *)
+  (*     |- context [ Pr [?C] ] => *)
+  (*     let H := fresh "H" in *)
+  (*     assert (Pr [C] == 1) as H; *)
+  (*       [|rewrite H; clear H] *)
+  (*   end. *)
+  (*   { *)
+  (*     fcf_irr_l; fcf_well_formed; fcf_irr_l; fcf_well_formed; fcf_compute. *)
+  (*   } *)
 
-  lazymatch goal with
-    |- context [ Pr [?C] ] =>
-    let H := fresh "H" in
-    assert (Pr [C] == 0) as H;
-    [|rewrite H; clear H]
-  end.
-    {
-      fcf_irr_l; fcf_well_formed; fcf_irr_l; fcf_well_formed; fcf_compute.
-    }
-    {
-      lazymatch goal with |- ?a <= ?b => change (a <= 1) end.
-      apply rat_le_1.
-      apply expnat_ge_1.
-      omega.
-    }
-  Admitted.
-    (* fcf_compute. *)
-    (* Unset Printing Notations. *)
-    (* Show. *)
+  (* lazymatch goal with *)
+  (*   |- context [ Pr [?C] ] => *)
+  (*   let H := fresh "H" in *)
+  (*   assert (Pr [C] == 0) as H; *)
+  (*   [|rewrite H; clear H] *)
+  (* end. *)
+  (*   { *)
+  (*     fcf_irr_l; fcf_well_formed; fcf_irr_l; fcf_well_formed; fcf_compute. *)
+  (*   } *)
+  (*   { *)
+  (*     lazymatch goal with |- ?a <= ?b => change (a <= 1) end. *)
+  (*     apply rat_le_1. *)
+  (*     apply expnat_ge_1. *)
+  (*     omega. *)
+  (*   } *)
+  (* Admitted. *)
 
-    (* fcf_simp. *)
+  (* Context {message list_message rand : base_type}. *)
 
-    (* SearchAbout Rat. *)
+  (* Context (Plaintext Ciphertext Key : DataTypeFamily). *)
+  (* Context {base_type : Set} {interp_base_type:base_type->Set}. *)
+  (* Inductive type := Type_base (t:base_type) | Type_arrow (dom:type) (cod:type). *)
+  (* Context {base_type : Set} {interp_base_type:base_type->Set}. *)
 
-    (* SearchAbout Rat refl. *)
+  (* Check term rand. *)
 
-    (* fcf_irr_r. *)
-    (* Print RatRel. *)
-    (* constructor; eauto. *)
-  (* Context (KeyGen : forall n, term rand -> Key n). *)
-  (* Context (Encrypt : forall n, Key n -> Plaintext n -> term rand -> Ciphertext n). *)
-  (* Context (Decrypt : forall n, Key n -> Ciphertext n -> Plaintext n). *)
-
-  (* Context (admissible_A1: pred_oc_fam). *)
-  (* Context (admissible_A2: pred_oc_func_2_fam). *)
 
   (* Lemma indist_encrypt : *)
   (*   forall n (p0 p1 : term Plaintext n) (n0 n1 : nat), *)
@@ -247,7 +236,9 @@ Section CompInterp.
 Section SymbolicProof.
   Context {base_type : Set} {interp_base_type : base_type -> Set}.
   Local Coercion type_base (t:base_type) : type base_type := Type_base t.
+  Context (Plaintext Ciphertext Key : DataTypeFamily).
   Context {message list_message rand bool : base_type}.
+
   Local Notation term := (term interp_base_type message list_message rand).
   Context (indist : forall {t : type base_type}, term t -> term t -> Prop). Arguments indist {_} _ _.
 
@@ -259,6 +250,23 @@ Section SymbolicProof.
   Lemma indist_if_then_else_rand_l (b:term bool) (x y:nat) :
     indist (Term_app (Term_app (Term_app if_then_else b) (Term_random x)) (Term_random y)) (Term_random x).
   Proof. exact (indist_if_then_else_irrelevant_l _ _ _ (indist_rand x y) _). Qed.
+
+  Context {forall n, Plaintext n : base_type}.
+
+  Context (KeyGen : forall n, term rand -> Key n).
+
+  Context (Encrypt : forall n, Key n -> Plaintext n -> term rand -> Ciphertext n).
+  Context (Decrypt : forall n, Key n -> Ciphertext n -> Plaintext n).
+
+  Context (admissible_A1: pred_oc_fam).
+  Context (admissible_A2: pred_oc_func_2_fam).
+
+  Lemma indist_encrypt :
+    forall n (p0 p1 : term (Plaintext n)) (n0 n1 : nat),
+      n0 <> n1 ->
+      indist (Term_app (Term_const (Encrypt n)) ((Term_const (KeyGen n)) p0 (Term_random n0))) (Term_app (Term_const (Encrypt n)) ((Term_const (KeyGen n)) p1 (Term_random n1))).
+
+  (* Lemma indist_refl {t} (x:term t) : indist x x. *)
 End SymbolicProof.
 
 Definition if_then_else {t : type base_type}
@@ -302,7 +310,6 @@ Proof.
   { eapply Proper_evalDist. eapply G. reflexivity. }
 Qed.
 
-
 Lemma Rnd_split_equiv n1 n2 : Comp_eq
     (x <-$ { 0 , 1 }^ n1 + n2; ret splitVector n1 n2 x)
     (x1 <-$ { 0 , 1 }^ n1; x2 <-$ { 0 , 1 }^ n2; ret (x1, x2)).
@@ -332,26 +339,27 @@ Lemma Comp_eq_evalDist A (x y:Comp A) :
   intro b.
   apply H1.
 Qed.
+
+  Lemma list_vector_split a b (T : Set) (x : Vector.t T _) : skipn (b) (Vector.to_list x) = Vector.to_list (snd (splitVector (b) a x)).
+    induction b; simpl; intuition.
+    destruct (splitVector b a (Vector.tl x)) eqn:?.
+    specialize (IHb (Vector.tl x)).
+    rewrite Heqp in IHb.
+    simpl in *.
+    rewrite <- IHb.
+    SearchAbout Vector.hd Vector.tl.
+    rewrite (Vector.eta x).
+    reflexivity.
+  Qed.
 (* Lemma Comp_eq_impl_evalDist A (x y : Comp A): *)
 (*   Comp_eq x y -> *)
 (*   evalDist *)
 Print Distribution.
 
 Axiom random_size : nat -> nat.
-Goal False.
 
-  (* pose_proof (forall t (x : term t), indist x x) as H. *)
-
-  (* pose proof (fun A B => indist_if_then_else_rand_l (bool:=BaseType_bool) (@indist random_size) (fun _ => Term_const if_then_else) A B) as H. *)
-
-  pose proof (fun A B => indist_if_then_else_rand_l (bool:=BaseType_bool) (@indist random_size) (fun _ => Term_const if_then_else) A B) as H.
-  match type of H with ?A -> ?C => assert A as HA; [clear H|specialize(H HA);clear HA] end.
-
-(* 2 subgoals, subgoal 1 (ID 30) *)
-  
-(*   ============================ *)
-(*   forall x y : nat, x <> y -> indist id (Term_random x) (Term_random y) *)
-
+Lemma indist_rand: forall x y : nat, indist random_size (Term_random x) (Term_random y).
+Proof.
   cbv [rand_end indist universal_security_game comp_interp_term interp_term]. (* to monadic probability notation *)
   intros.
   pose proof negligible_const_num 1.
@@ -401,69 +409,36 @@ Goal False.
       }
     }
   }
-  Admitted.
+  etransitivity.
+  etransitivity.
+  2: apply H2.
 
+  fcf_inline_first.
+    (*   |- context [ Pr [?C] ] => *)
+    (*   let H := fresh "H" in *)
+    (*   assert (Pr [C] == 1) as H; *)
+    (*     [|rewrite H; clear H] *)
+    (* end. *)
+  (* match goal with |- context [S ?x * D] => replace (S x * D)%nat with (x * D + D)%nat by ring end. *)
+  replace (S x * D)%nat with (x * D + D)%nat by ring.
+  fcf_skip.
+  fcf_simp.
+  apply evalDist_ret_eq.
+  repeat f_equal.
+  rewrite list_vector_split.
+  eapply firstn_ge_all.
+  rewrite to_list_length.
+  auto.
 
-(* 2 subgoals, subgoal 1 (ID 34) *)
-  
-(*   ============================ *)
-(*   forall x y : nat, *)
-(*   x <> y -> *)
-(*   forall (l : nat -> nat) (adv : nat -> list bool -> list (list bool) -> list bool) *)
-(*     (dst : forall t : type base_type, nat -> list bool -> interp_type interp_base_type t -> bool), *)
-(*   negligible *)
-(*     (fun eta : nat => *)
-(*      | *)
-(*      Pr [good_rand_tape' <-$ { 0 , 1 }^ S x * id eta; *)
-(*          evil_rand_tape' <-$ { 0 , 1 }^ l eta; *)
-(*          ret dst (Type_base BaseType_message) eta (Vector.to_list evil_rand_tape') *)
-(*                (interp_term *)
-(*                   (fun n : nat => firstn (id eta) (skipn (n * id eta) (Vector.to_list good_rand_tape'))) *)
-(*                   (adv eta (Vector.to_list evil_rand_tape')) (Term_random x)) ] - *)
-(*      Pr [good_rand_tape' <-$ { 0 , 1 }^ S y * id eta; *)
-(*          evil_rand_tape' <-$ { 0 , 1 }^ l eta; *)
-(*          ret dst (Type_base BaseType_message) eta (Vector.to_list evil_rand_tape') *)
-(*                (interp_term *)
-(*                   (fun n : nat => firstn (id eta) (skipn (n * id eta) (Vector.to_list good_rand_tape'))) *)
-(*                   (adv eta (Vector.to_list evil_rand_tape')) (Term_random y)) ] |) *)
-
-  (* This probably could be proven in this form -- the argument is that the two subsequences of the good random tape that are given to [dst] are non-overlapping. *)
-
-  
-  (* simpl. (* to raw probability equations *) *)
-  
-(* 2 subgoals, subgoal 1 (ID 141) *)
-  
-(*   ============================ *)
-(*   forall x y : nat, *)
-(*   x <> y -> *)
-(*   forall l : nat -> nat, *)
-(*   (nat -> list bool -> list (list bool) -> list bool) -> *)
-(*   forall dst : forall t : type base_type, nat -> list bool -> interp_type interp_base_type t -> bool, *)
-(*   negligible *)
-(*     (fun eta : nat => *)
-(*      | *)
-(*      sumList (getAllBvectors (id eta + x * id eta)) *)
-(*        (fun b : Bvector (id eta + x * id eta) => *)
-(*         1 / expnat 2 (id eta + x * id eta) * *)
-(*         sumList (getAllBvectors (l eta)) *)
-(*           (fun b0 : Bvector (l eta) => *)
-(*            1 / expnat 2 (l eta) * *)
-(*            (if *)
-(*              EqDec_dec bool_EqDec *)
-(*                (dst (Type_base BaseType_message) eta (Vector.to_list b0) *)
-(*                   (firstn (id eta) (skipn (x * id eta) (Vector.to_list b)))) true *)
-(*             then 1 *)
-(*             else 0))) - *)
-(*      sumList (getAllBvectors (id eta + y * id eta)) *)
-(*        (fun b : Bvector (id eta + y * id eta) => *)
-(*         1 / expnat 2 (id eta + y * id eta) * *)
-(*         sumList (getAllBvectors (l eta)) *)
-(*           (fun b0 : Bvector (l eta) => *)
-(*            1 / expnat 2 (l eta) * *)
-(*            (if *)
-(*              EqDec_dec bool_EqDec *)
-(*                (dst (Type_base BaseType_message) eta (Vector.to_list b0) *)
-(*                   (firstn (id eta) (skipn (y * id eta) (Vector.to_list b)))) true *)
-(*             then 1 *)
-(*             else 0))) |) *)
+  fcf_inline_first.
+  replace (S y * D)%nat with (y * D + D)%nat by ring.
+  fcf_skip.
+  fcf_simp.
+  apply evalDist_ret_eq.
+  repeat f_equal.
+  rewrite list_vector_split.
+  symmetry.
+  eapply firstn_ge_all.
+  rewrite to_list_length.
+  auto.
+Qed.
